Some progress on type checking safe functions

src/test/Manifest.fst
@@ -1,36 +1,50 @@
 module Manifest
-open FStar.UInt64
 
-type uint64 = FStar.UInt64.t
+let nat64_max = 0x10000000000000000
+type nat64 = i:nat{i <= nat64_max}
 
 type argtype =
-  | AInt : argtype
+  | ANat64 : argtype
   | AChar: argtype
   
 type calltable_entry =
-  |Mkcalltable_entry : fname:string -> fstart_address : int -> fsize:int -> args: (list argtype) -> calltable_entry
+  |Mkcalltable_entry : fname:string -> fstart_address : nat64 -> fsize:nat64 -> args: (list argtype) -> calltable_entry
 
 type calltable = 
-  | MkCalltable : calltable_start:int -> calltable_size: uint64 -> entries: (list calltable_entry) -> calltable
+  | MkCalltable : calltable_start:nat64 -> calltable_size: nat64 -> entries: (list calltable_entry) -> calltable
 
 type umemlayout =
- | MkUmemlayout :  u_start:uint64 -> u_size:uint64 ->
-                   bitmap_address:uint64 -> bitmap_size:uint64 ->
+ | MkUmemlayout :  base_start:nat64 -> base_size:nat64 ->
+                   bitmap_address:nat64 -> bitmap_size:nat64 ->
 		   ctable: calltable ->
-		   code_start:uint64 -> code_size: uint64 ->
-		   heap_start: uint64 -> heap_and_stack_size:uint64 ->
-		   stack_start:uint64 -> umemlayout
+		   code_start:nat64 -> code_size: nat64 ->
+		   heap_start: nat64 -> heap_size:nat64 ->
+		   stack_start:nat64 -> stack_size:nat64 -> umemlayout
 
 
-let get_u_start (m:umemlayout) = m.u_start
-let get_u_size (m:umemlayout) = m.u_size
+val get_u_start (m:umemlayout) : (r:nat64)
+let get_u_start (m:umemlayout) = m.code_start
+let get_u_size (m:umemlayout) = m.code_size + m.heap_size + m.stack_size
+let get_u_end (m:umemlayout) = m.stack_start
+
+val get_bitmap_start (m:umemlayout) : (r:nat64)
 let get_bitmap_start (m:umemlayout) = m.bitmap_address
+let get_bitmap_size (m:umemlayout) = m.bitmap_size
+
 let get_calltable_start (m:umemlayout) = m.ctable.calltable_start
 let get_code_start (m:umemlayout) = m.code_start
+let get_code_size (m:umemlayout) = m.code_size
+
 let get_heap_start (m:umemlayout) = m.heap_start
+let get_heap_size (m:umemlayout) = m.heap_size
 let get_stack_start (m:umemlayout) = m.stack_start
+let get_stack_size (m:umemlayout) = m.stack_size
 
-let address_within_procedure (fname:string) (dst:int) (env:umemlayout) = true
+let address_within_procedure (fname:string) (dst:nat64) (env:umemlayout) = true
 
-val is_inside_u_region (addr:uint64) (u:umemlayout) : bool
-let is_inside_u_region (addr:uint64) (u:umemlayout) = ( addr <^ ((get_u_start u) +^ (get_u_size u))) && ( addr >=^ (get_u_start u))  
+val is_inside_u_region (addr:nat64) (u:umemlayout) : bool
+let is_inside_u_region (addr:nat64) (u:umemlayout) = ( addr < ((get_u_start u) + (get_u_size u))) && ( addr >= (get_u_start u))  
+
+(* fix the definitions later *)
+let is_known_verified_entryponat6464 (faddr:nat64) (u:umemlayout) = true
+let is_known_untrusted_entryponat6464 (faddr:nat64) (u:umemlayout) = true
